refactor(Propositional): Redesign Hilbert Systems (#812)

Foundation/Propositional/FMT/Completeness.lean
@@ -1,6 +1,6 @@
 module
 
-public import Foundation.Propositional.FMT.Hilbert
+public import Foundation.Propositional.FMT.Hilbert.Basic
 public import Foundation.Propositional.Hilbert.WF_VF
 
 @[expose] public section
@@ -9,7 +9,8 @@ namespace LO.Propositional
 
 open Entailment.Corsi
 
-variable {L : Logic ℕ}
+variable {S} [Entailment S (Formula ℕ)]
+         {𝓢 : S}
 
 abbrev SubformulaOf (φ : Formula ℕ) : Type := { ψ // ψ ∈ φ.subformulas }
 instance : Fintype (SubformulaOf φ) where
@@ -24,9 +25,9 @@ namespace HintikkaPair
 
 variable {H : HintikkaPair φ}
 
-def Consistent (L : Logic ℕ) (H : HintikkaPair φ) : Prop := L ⊬ Finset.conj' H.1 (·.1) 🡒 (⩖ x ∈ H.2, ↑x)
-lemma iff_consistent : H.Consistent L ↔ ¬(L ⊢ Finset.conj' H.1 (·.1) 🡒 (⩖ x ∈ H.2, ↑x)) := by simp [Consistent];
-lemma iff_not_consistent : ¬(H.Consistent L) ↔ L ⊢ Finset.conj' H.1 (·.1) 🡒 (⩖ x ∈ H.2, ↑x) := by simp [Consistent];
+def Consistent (𝓢 : S) (H : HintikkaPair φ) : Prop := 𝓢 ⊬ (⩕ x ∈ H.1, ↑x) 🡒 (⩖ x ∈ H.2, ↑x)
+lemma iff_consistent : H.Consistent 𝓢 ↔ (𝓢 ⊬ (⩕ x ∈ H.1, ↑x) 🡒 (⩖ x ∈ H.2, ↑x)) := by simp [Consistent];
+lemma iff_not_consistent : ¬(H.Consistent 𝓢) ↔ 𝓢 ⊢ (⩕ x ∈ H.1, ↑x) 🡒 (⩖ x ∈ H.2, ↑x) := by simp [Consistent];
 
 @[grind]
 def Saturated (H : HintikkaPair φ) := H.1 ∪ H.2 = Finset.univ
@@ -44,12 +45,12 @@ lemma mem₂_of_not_mem₁_of_saturated (h : H.Saturated) : ψ ∉ H.1 → ψ �
 def insert₁ (H : HintikkaPair φ) (ψ : { ψ // ψ ∈ φ.subformulas }) : HintikkaPair φ := ⟨insert ψ H.1, H.2⟩
 def insert₂ (H : HintikkaPair φ) (ψ : { ψ // ψ ∈ φ.subformulas }) : HintikkaPair φ := ⟨H.1, insert ψ H.2⟩
 
-variable [Entailment.VF L]
+variable [Entailment.VF 𝓢]
 
 @[grind ⇒]
 lemma either_consistent_insert
-  (H_consis : H.Consistent L) (ψ)
-  : Consistent L (H.insert₁ ψ) ∨ Consistent L (H.insert₂ ψ) := by
+  (H_consis : H.Consistent 𝓢) (ψ)
+  : Consistent 𝓢 (H.insert₁ ψ) ∨ Consistent 𝓢 (H.insert₂ ψ) := by
   contrapose! H_consis;
   apply iff_not_consistent.mpr;
 
@@ -61,18 +62,18 @@ lemma either_consistent_insert
   let Δ₀ : Formula ℕ := ⩖ δ ∈ H.2, ↑δ;
   let Δ₁ : Formula ℕ := ⩖ δ ∈ (H.insert₂ ψ).2, ↑δ;
 
-  replace h₁ : L ⊢ Γ₁ 🡒 Δ₀ := iff_not_consistent.mp h₁;
-  replace h₂ : L ⊢ Γ₀ 🡒 Δ₁ := iff_not_consistent.mp h₂;
-  show L ⊢ Γ₀ 🡒 Δ₀;
+  replace h₁ : 𝓢 ⊢ Γ₁ 🡒 Δ₀ := iff_not_consistent.mp h₁;
+  replace h₂ : 𝓢 ⊢ Γ₀ 🡒 Δ₁ := iff_not_consistent.mp h₂;
+  show 𝓢 ⊢ Γ₀ 🡒 Δ₀;
 
   apply ruleI ?_ $ ruleD impId h₁;
-  show L ⊢ Γ₀ 🡒 Δ₀ ⋎ Γ₁;
+  show 𝓢 ⊢ Γ₀ 🡒 Δ₀ ⋎ Γ₁;
 
   apply ruleI $ ruleC h₂ orIntroR;
-  show L ⊢ Δ₁ ⋏ (Δ₀ ⋎ Γ₀) 🡒 Δ₀ ⋎ Γ₁;
+  show 𝓢 ⊢ Δ₁ ⋏ (Δ₀ ⋎ Γ₀) 🡒 Δ₀ ⋎ Γ₁;
 
   apply C_replace_both;
-  . show L ⊢ (Δ₀ ⋎ ↑ψ) ⋏ (Δ₀ ⋎ Γ₀) 🡒 Δ₀ ⋎ ↑ψ ⋏ Γ₀;
+  . show 𝓢 ⊢ (Δ₀ ⋎ ↑ψ) ⋏ (Δ₀ ⋎ Γ₀) 🡒 Δ₀ ⋎ ↑ψ ⋏ Γ₀;
     exact collectOrAnd;
   . apply ruleC ?_ andElimR;
     apply ruleI andElimL;
@@ -99,71 +100,71 @@ namespace lindenbaum
 
 open Classical
 
-variable {L : Logic ℕ} {φ : Formula ℕ} {H : HintikkaPair φ}
+variable {𝓢 : S} {φ : Formula ℕ} {H : HintikkaPair φ}
 
-noncomputable def next (L : Logic ℕ) (ψ : SubformulaOf φ) (H : HintikkaPair φ) : HintikkaPair φ :=
-  if Consistent L (H.insert₁ ψ) then H.insert₁ ψ else H.insert₂ ψ
+noncomputable def next (𝓢 : S) (ψ : SubformulaOf φ) (H : HintikkaPair φ) : HintikkaPair φ :=
+  if Consistent 𝓢 (H.insert₁ ψ) then H.insert₁ ψ else H.insert₂ ψ
 
-variable [Entailment.VF L]
-
-lemma next_consistent (H_consis : H.Consistent L) : (next L ψ H).Consistent L := by
-  by_cases h : Consistent L (H.insert₁ ψ) <;>
+variable [Entailment.VF 𝓢] in
+lemma next_consistent (H_consis : H.Consistent 𝓢) : (next 𝓢 ψ H).Consistent 𝓢 := by
+  by_cases h : Consistent 𝓢 (H.insert₁ ψ) <;>
   . dsimp [next, h];
     grind;
 
-lemma next_monotone₁ : H.1 ⊆ (next L ψ H).1 := by
+lemma next_monotone₁ : H.1 ⊆ (next 𝓢 ψ H).1 := by
   simp [next, insert₁, insert₂];
   split <;> grind;
 
-lemma next_monotone₂ : H.2 ⊆ (next L ψ H).2 := by
+lemma next_monotone₂ : H.2 ⊆ (next 𝓢 ψ H).2 := by
   simp [next, insert₁, insert₂];
   split <;> grind;
 
-lemma next_either_mem (ψ) : ψ ∈ (next L ψ H).1 ∨ ψ ∈ (next L ψ H).2 := by
+lemma next_either_mem (ψ) : ψ ∈ (next 𝓢 ψ H).1 ∨ ψ ∈ (next 𝓢 ψ H).2 := by
   simp [next, insert₁, insert₂];
   split <;> grind;
 
-noncomputable def enum (L : Logic ℕ) (H : HintikkaPair φ) : List (SubformulaOf φ) → HintikkaPair φ
+noncomputable def enum (𝓢 : S) (H : HintikkaPair φ) : List (SubformulaOf φ) → HintikkaPair φ
   | [] => H
-  | ψ :: Δ => next L ψ (enum L H Δ)
+  | ψ :: Δ => next 𝓢 ψ (enum 𝓢 H Δ)
 
-lemma enum_consistent (H_consis : H.Consistent L) (Γ : List (SubformulaOf φ)) : (enum L H Γ).Consistent L := by
+variable [Entailment.VF 𝓢] in
+lemma enum_consistent (H_consis : H.Consistent 𝓢) (Γ : List (SubformulaOf φ)) : (enum 𝓢 H Γ).Consistent 𝓢 := by
   induction Γ with
   | nil => assumption;
   | cons ψ Γ ih => apply next_consistent; exact ih;
 
-lemma enum_monotone₁ {Γ : List (SubformulaOf φ)} : H.1 ⊆ (enum L H Γ).1 := by
+lemma enum_monotone₁ {Γ : List (SubformulaOf φ)} : H.1 ⊆ (enum 𝓢 H Γ).1 := by
   induction Γ with
   | nil => simp [enum];
   | cons ψ Γ ih =>
-    trans (enum L H Γ).1;
+    trans (enum 𝓢 H Γ).1;
     . exact ih;
     . apply next_monotone₁
 
-lemma enum_monotone₂ {Γ : List (SubformulaOf φ)} : H.2 ⊆ (enum L H Γ).2 := by
+lemma enum_monotone₂ {Γ : List (SubformulaOf φ)} : H.2 ⊆ (enum 𝓢 H Γ).2 := by
   induction Γ with
   | nil => simp [enum];
   | cons ψ Γ ih =>
-    trans (enum L H Γ).2;
+    trans (enum 𝓢 H Γ).2;
     . exact ih;
     . apply next_monotone₂
 
-lemma enum_of_mem (hψ : ψ ∈ Γ) : ψ ∈ (enum L H Γ).1 ∨ ψ ∈ (enum L H Γ).2 := by
+lemma enum_of_mem (hψ : ψ ∈ Γ) : ψ ∈ (enum 𝓢 H Γ).1 ∨ ψ ∈ (enum 𝓢 H Γ).2 := by
   induction Γ with
   | nil => simp at hψ;
   | cons χ Δ ih =>
     simp only [List.mem_cons] at hψ;
     rcases hψ with rfl | hψ;
-    . rcases next_either_mem (L := L) (H := enum L H Δ) ψ with h | h;
+    . rcases next_either_mem (𝓢 := 𝓢) (H := enum 𝓢 H Δ) ψ with h | h;
       . left; simpa [enum];
       . right; simpa [enum];
     . rcases ih hψ with h | h;
       . left; apply next_monotone₁ h;
       . right; apply next_monotone₂ h;
 
-noncomputable def sat (L : Logic ℕ) (H : HintikkaPair φ) : HintikkaPair φ := enum L H Finset.univ.toList
+noncomputable def sat (𝓢 : S) (H : HintikkaPair φ) : HintikkaPair φ := enum 𝓢 H Finset.univ.toList
 
-lemma sat_saturated : (sat L H).Saturated := by
+lemma sat_saturated : (sat 𝓢 H).Saturated := by
   ext ψ;
   simp only [Finset.univ_eq_attach, Finset.mem_union, Finset.mem_attach, iff_true];
   apply enum_of_mem;
@@ -172,8 +173,8 @@ lemma sat_saturated : (sat L H).Saturated := by
 end lindenbaum
 
 open lindenbaum in
-lemma lindenbaum (H : HintikkaPair φ) (H_consis : H.Consistent L) : ∃ H' : HintikkaPair φ, H.1 ⊆ H'.1 ∧ H.2 ⊆ H'.2 ∧ H'.Consistent L ∧ H'.Saturated := by
-  use lindenbaum.sat L H;
+lemma lindenbaum (H : HintikkaPair φ) (H_consis : H.Consistent 𝓢) : ∃ H' : HintikkaPair φ, H.1 ⊆ H'.1 ∧ H.2 ⊆ H'.2 ∧ H'.Consistent 𝓢 ∧ H'.Saturated := by
+  use lindenbaum.sat 𝓢 H;
   refine ⟨?_, ?_, ?_, ?_⟩;
   . apply enum_monotone₁;
   . apply enum_monotone₂;
@@ -182,35 +183,34 @@ lemma lindenbaum (H : HintikkaPair φ) (H_consis : H.Consistent L) : ∃ H' : Hi
 
 end HintikkaPair
 
-abbrev ConsistentSaturatedHintikkaPair (L) (φ) := { H : HintikkaPair φ // H.Consistent L ∧ H.Saturated }
+abbrev ConsistentSaturatedHintikkaPair (𝓢 : S) (φ) := { H : HintikkaPair φ // H.Consistent 𝓢 ∧ H.Saturated }
 
 namespace ConsistentSaturatedHintikkaPair
 
-variable {H : ConsistentSaturatedHintikkaPair L φ}
+variable {H : ConsistentSaturatedHintikkaPair 𝓢 φ}
 
 open Formula
 
-variable [Entailment.VF L]
-
-lemma lindenbaum (H : HintikkaPair φ) (H_consis : H.Consistent L) : ∃ H' : ConsistentSaturatedHintikkaPair L φ, H.1 ⊆ H'.1.1 ∧ H.2 ⊆ H'.1.2 := by
+variable [Entailment.VF 𝓢] in
+lemma lindenbaum (H : HintikkaPair φ) (H_consis : H.Consistent 𝓢) : ∃ H' : ConsistentSaturatedHintikkaPair 𝓢 φ, H.1 ⊆ H'.1.1 ∧ H.2 ⊆ H'.1.2 := by
   obtain ⟨H', _, _, H'_consis, H'_saturated⟩ := HintikkaPair.lindenbaum H H_consis;
   use ⟨H', ⟨H'_consis, H'_saturated⟩⟩;
 
-@[simp, grind .] lemma consistent (H : ConsistentSaturatedHintikkaPair L φ) : HintikkaPair.Consistent L H.1 := H.2.1
-@[simp, grind .] lemma saturated (H : ConsistentSaturatedHintikkaPair L φ) : HintikkaPair.Saturated H.1 := H.2.2
+@[simp, grind .] lemma consistent (H : ConsistentSaturatedHintikkaPair 𝓢 φ) : HintikkaPair.Consistent 𝓢 H.1 := H.2.1
+@[simp, grind .] lemma saturated (H : ConsistentSaturatedHintikkaPair 𝓢 φ) : HintikkaPair.Saturated H.1 := H.2.2
+
+variable [Entailment.VF 𝓢]
 
 @[grind .]
 lemma not_mem_both : ¬(ψ ∈ H.1.1 ∧ ψ ∈ H.1.2) := by
   by_contra! hC;
-  obtain ⟨h₁, h₂⟩ := hC;
+  rcases hC with ⟨h₁, h₂⟩;
   apply H.consistent;
   apply C_replace_both;
-  . show L ⊢ ψ.1 🡒 ψ.1;
+  . show 𝓢 ⊢ ψ.1 🡒 ψ.1;
     exact impId;
-  . apply mem_fconj';
-    grind;
-  . apply mem_fdisj';
-    grind;
+  . apply mem_fconj'; grind;
+  . apply mem_fdisj'; grind;
 
 @[grind =]
 lemma iff_mem₁_not_mem₂ : ψ ∈ H.1.1 ↔ ψ ∉ H.1.2 := by
@@ -226,9 +226,7 @@ lemma iff_mem₂_not_mem₁ : ψ ∈ H.1.2 ↔ ψ ∉ H.1.1 := by
     apply not_mem_both hC.symm;
   . apply HintikkaPair.mem₂_of_not_mem₁_of_saturated H.saturated;
 
-
-
-lemma imp_closed (hSψ : ψ ∈ φ.subformulas) (hSχ : χ ∈ φ.subformulas) : L ⊢ ψ 🡒 χ → ⟨ψ, hSψ⟩ ∈ H.1.1 → ⟨χ, hSχ⟩ ∈ H.1.1 := by
+lemma imp_closed (hSψ : ψ ∈ φ.subformulas) (hSχ : χ ∈ φ.subformulas) : 𝓢 ⊢ ψ 🡒 χ → ⟨ψ, hSψ⟩ ∈ H.1.1 → ⟨χ, hSχ⟩ ∈ H.1.1 := by
   rintro h₁ hφ;
   by_contra hψ;
   replace hψ := iff_mem₂_not_mem₁.mpr hψ;
@@ -252,10 +250,8 @@ lemma mem_top (h : ⊤ ∈ φ.subformulas) : ⟨⊤, h⟩ ∈ H.1.1 := by
   by_contra hC;
   apply H.consistent;
   apply ruleI (ψ := ⊤);
-  . apply af;
-    exact Entailment.verum!;
-  . apply mem_fdisj';
-    grind;
+  . apply af; simp;
+  . apply mem_fdisj'; grind;
 
 lemma iff_mem_and (hSub : ψ ⋏ χ ∈ φ.subformulas) : ⟨ψ ⋏ χ, hSub⟩ ∈ H.1.1 ↔ ⟨ψ, subformulas.mem_and hSub |>.1⟩ ∈ H.1.1 ∧ ⟨χ, subformulas.mem_and hSub |>.2⟩ ∈ H.1.1 := by
   constructor;
@@ -268,7 +264,7 @@ lemma iff_mem_and (hSub : ψ ⋏ χ ∈ φ.subformulas) : ⟨ψ ⋏ χ, hSub⟩ 
     replace hψχ := iff_mem₂_not_mem₁.mpr hψχ;
     apply H.consistent;
     apply C_replace_both;
-    . show L ⊢ ψ ⋏ χ 🡒 ψ ⋏ χ;
+    . show 𝓢 ⊢ ψ ⋏ χ 🡒 ψ ⋏ χ;
       exact impId;
     . apply ruleC <;>
       . apply mem_fconj';
@@ -285,7 +281,7 @@ lemma iff_mem_or (hSub : ψ ⋎ χ ∈ φ.subformulas) : ⟨ψ ⋎ χ, hSub⟩ �
     replace hψ := iff_mem₂_not_mem₁.mpr hψ;
     apply H.consistent;
     apply C_replace_both;
-    . show L ⊢ ψ ⋎ χ 🡒 ψ ⋎ χ;
+    . show 𝓢 ⊢ ψ ⋎ χ 🡒 ψ ⋎ χ;
       exact impId;
     . apply mem_fconj';
       grind;
@@ -303,34 +299,35 @@ namespace FMT
 
 open Formula
 
-variable [Entailment.VF L] [Entailment.Disjunctive L] [Entailment.Consistent L]
+variable [Entailment.VF 𝓢] [Entailment.Disjunctive 𝓢] [Entailment.Consistent 𝓢]
 
 open Classical in
-noncomputable def HintikkaModel (L : Logic ℕ) [Entailment.VF L] [Entailment.Consistent L] [Entailment.Disjunctive L] (φ : Formula ℕ) : FMT.Model :=
+noncomputable def HintikkaModel (𝓢 : S) [Entailment.VF 𝓢] [Entailment.Consistent 𝓢] [Entailment.Disjunctive 𝓢] (φ : Formula ℕ) : FMT.Model :=
   letI H₀ : HintikkaPair φ := ⟨
     ∅,
-    Finset.univ.filter (λ ⟨δ, hδ⟩ => ∃ χ ξ, δ = χ.1 🡒 ξ.1 ∧ ∃ H : ConsistentSaturatedHintikkaPair L φ, χ ∈ H.1.1 ∧ ξ ∈ H.1.2 )
+    Finset.univ.filter (λ ⟨δ, hδ⟩ => ∃ χ ξ, δ = χ.1 🡒 ξ.1 ∧ ∃ H : ConsistentSaturatedHintikkaPair 𝓢 φ, χ ∈ H.1.1 ∧ ξ ∈ H.1.2 )
   ⟩;
-  haveI hH₀ := ConsistentSaturatedHintikkaPair.lindenbaum (φ := φ) (L := L) H₀ $ by
+  haveI hH₀ := ConsistentSaturatedHintikkaPair.lindenbaum H₀ $ by
+    show H₀.Consistent 𝓢;
     apply HintikkaPair.iff_consistent.mpr;
     by_contra! hC;
-    have : L ⊢ ⩖ δ ∈ H₀.2, ↑δ := hC ⨀ by simp [H₀];
-    obtain ⟨δ, hδ₁, hδ₂⟩ : ∃ δ ∈ H₀.2, L ⊢ ↑δ := by
+    have : 𝓢 ⊢ ⩖ δ ∈ H₀.2, ↑δ := hC ⨀ by simp [H₀];
+    obtain ⟨δ, hδ₁, hδ₂⟩ : ∃ δ ∈ H₀.2, 𝓢 ⊢ ↑δ := by
       apply DP_fdisj;
       apply Entailment.mdp! hC;
       simp [H₀];
-    obtain ⟨χ, ξ, e, Γ, hΓχ, hΓξ⟩ : ∃ χ ξ : SubformulaOf φ, δ = χ.1 🡒 ξ.1 ∧ ∃ H : ConsistentSaturatedHintikkaPair L φ, χ ∈ H.1.1 ∧ ξ ∈ H.1.2  := by
+    obtain ⟨χ, ξ, e, Γ, hΓχ, hΓξ⟩ : ∃ χ ξ : SubformulaOf φ, δ = χ.1 🡒 ξ.1 ∧ ∃ H : ConsistentSaturatedHintikkaPair 𝓢 φ, χ ∈ H.1.1 ∧ ξ ∈ H.1.2  := by
       simpa [H₀] using hδ₁;
     apply Γ.consistent;
     apply C_replace_both;
-    . show L ⊢ χ.1 🡒 ξ.1;
+    . show 𝓢 ⊢ χ.1 🡒 ξ.1;
       exact e ▸ hδ₂;
     . apply mem_fconj';
       use χ;
     . apply mem_fdisj';
       use ξ;
   {
-    World := ConsistentSaturatedHintikkaPair L φ
+    World := ConsistentSaturatedHintikkaPair 𝓢 φ
     Rel ψ H I :=
       match ψ with
       | χ 🡒 ξ =>
@@ -347,12 +344,12 @@ noncomputable def HintikkaModel (L : Logic ℕ) [Entailment.VF L] [Entailment.Co
         rintro _;
         let χ' : SubformulaOf φ := ⟨χ, by grind⟩;
         let ξ' : SubformulaOf φ := ⟨ξ, by grind⟩;
-        by_cases h : ∀ I : ConsistentSaturatedHintikkaPair L φ, χ' ∈ I.1.2 ∨ ξ' ∈ I.1.1;
+        by_cases h : ∀ I : ConsistentSaturatedHintikkaPair 𝓢 φ, χ' ∈ I.1.2 ∨ ξ' ∈ I.1.1;
         . right;
           exact h I;
         . left;
           apply hH₀.choose_spec |>.2;
-          suffices ∃ χ' ξ', χ 🡒 ξ = χ'.1 🡒 ξ'.1 ∧ ∃ I : ConsistentSaturatedHintikkaPair L φ, χ' ∈ I.1.1 ∧ ξ' ∈ I.1.2 by
+          suffices ∃ χ' ξ', χ 🡒 ξ = χ'.1 🡒 ξ'.1 ∧ ∃ I : ConsistentSaturatedHintikkaPair 𝓢 φ, χ' ∈ I.1.1 ∧ ξ' ∈ I.1.2 by
             simpa only [H₀, Finset.univ_eq_attach, Finset.mem_filter, Finset.mem_attach, true_and] using this;
           push_neg at h;
           obtain ⟨I, hI₁, hI₂⟩ := h;
@@ -366,7 +363,7 @@ noncomputable def HintikkaModel (L : Logic ℕ) [Entailment.VF L] [Entailment.Co
   }
 
 open Formula.FMT in
-lemma HintikkaModel.truthlemma {H : HintikkaModel L φ} (hsub : ψ ∈ φ.subformulas) : ⟨ψ, hsub⟩ ∈ H.1.1 ↔ H ⊩ ψ := by
+lemma HintikkaModel.truthlemma {H : HintikkaModel 𝓢 φ} (hsub : ψ ∈ φ.subformulas) : ⟨ψ, hsub⟩ ∈ H.1.1 ↔ H ⊩ ψ := by
   induction ψ generalizing H with
   | hatom a => tauto;
   | hfalsum => simp;
@@ -383,8 +380,9 @@ lemma HintikkaModel.truthlemma {H : HintikkaModel L φ} (hsub : ψ ∈ φ.subfor
     . contrapose!;
       intro h;
       apply Forces.not_def_imp.mpr;
-      obtain ⟨I, hI₁, hI₂⟩ := ConsistentSaturatedHintikkaPair.lindenbaum (φ := φ) (L := L) ({⟨χ, by grind⟩}, {⟨ξ, by grind⟩}) $ by
-        suffices L ⊬ χ 🡒 ξ by simpa [HintikkaPair.Consistent];
+      obtain ⟨I, hI₁, hI₂⟩ := ConsistentSaturatedHintikkaPair.lindenbaum (φ := φ) ({⟨χ, by grind⟩}, {⟨ξ, by grind⟩}) $ by
+        show HintikkaPair.Consistent 𝓢 ({⟨χ, _⟩}, {⟨ξ, _⟩});
+        suffices 𝓢 ⊬ χ 🡒 ξ by simpa [HintikkaPair.Consistent];
         by_contra! hC;
         apply H.consistent;
         apply af;
@@ -394,22 +392,19 @@ lemma HintikkaModel.truthlemma {H : HintikkaModel L φ} (hsub : ψ ∈ φ.subfor
         use ⟨χ 🡒 ξ, by tauto⟩;
       use I;
       refine ⟨?_, ?_, ?_⟩;
-      . dsimp [HintikkaModel]
-        grind;
-      . apply ihχ (by grind) |>.mp;
-        grind;
-      . apply ihξ (by grind) |>.not.mp;
-        apply ConsistentSaturatedHintikkaPair.iff_mem₂_not_mem₁.mp;
-        grind;
+      . dsimp [HintikkaModel]; grind;
+      . apply ihχ (by grind) |>.mp; grind;
+      . apply ihξ (by grind) |>.not.mp; grind;
 
 
 open Formula.FMT in
-theorem provable_of_validOnHintikkaModel : (HintikkaModel L φ) ⊧ φ → L ⊢ φ := by
+theorem provable_of_validOnHintikkaModel : (HintikkaModel 𝓢 φ) ⊧ φ → 𝓢 ⊢ φ := by
   contrapose!;
   intro h;
   apply ValidOnModel.not_of_exists_world;
-  obtain ⟨H, _, hH₂⟩ := ConsistentSaturatedHintikkaPair.lindenbaum (φ := φ) (L := L)  ⟨∅, {⟨φ, by grind⟩}⟩ $ by
-    suffices ¬L ⊢ ⊤ 🡒 φ by simpa [HintikkaPair.Consistent];
+  obtain ⟨H, _, hH₂⟩ := ConsistentSaturatedHintikkaPair.lindenbaum ⟨∅, {⟨φ, subformulas.mem_self⟩}⟩ $ by
+    show HintikkaPair.Consistent 𝓢 (∅, {⟨φ, _⟩});
+    suffices ¬𝓢 ⊢ ⊤ 🡒 φ by simpa [HintikkaPair.Consistent];
     contrapose! h;
     exact h ⨀ Entailment.verum!;
   use H;
