Foundation/Propositional/Kripke/AxiomKreiselPutnam.lean
@@ -33,7 +33,8 @@ variable {F : Kripke.Frame}
 
 open Formula (atom)
 
-lemma validate_axiomKreiselPutnam_of_satisfiesKreiselPutnamCondition [F.SatisfiesKreiselPutnamCondition ] : F ⊧ (Axioms.KreiselPutnam (.atom 0) (.atom 1) (.atom 2)) := by
+@[simp, grind .]
+lemma validate_axiomKreiselPutnam_of_satisfiesKreiselPutnamCondition [F.SatisfiesKreiselPutnamCondition ] : F ⊧ (Axioms.KreiselPutnam φ ψ χ) := by
   intro V x y Rxy h₁;
   by_contra hC;
   replace hC := Satisfies.or_def.not.mp hC;
@@ -61,7 +62,7 @@ lemma validate_axiomKreiselPutnam_of_satisfiesKreiselPutnamCondition [F.Satisfie
       . exfalso; exact hz₂₂ h;
   ⟩;
 
-  have : ¬Satisfies ⟨F, V⟩ u (∼(.atom 0)) := by
+  have : ¬Satisfies ⟨F, V⟩ u (∼φ) := by
     by_contra hC;
     rcases Satisfies.or_def.mp $ h₁ Ryu hC with (h | h);
     . apply hz₁₂; exact Satisfies.formula_hereditary Ruz₁ h;
@@ -71,8 +72,8 @@ lemma validate_axiomKreiselPutnam_of_satisfiesKreiselPutnamCondition [F.Satisfie
   obtain ⟨v, Ruv, hv⟩ := this;
 
   obtain ⟨w, Rvw, (Rz₁w | Rz₂w)⟩ := h v Ruv;
-  . exact Satisfies.not_of_neg (Satisfies.formula_hereditary (φ := (∼(.atom 0))) Rz₁w hz₁₁) $ Satisfies.formula_hereditary Rvw hv;
-  . exact Satisfies.not_of_neg (Satisfies.formula_hereditary (φ := (∼(.atom 0))) Rz₂w hz₂₁) $ Satisfies.formula_hereditary Rvw hv;
+  . exact Satisfies.not_of_neg (Satisfies.formula_hereditary (φ := (∼φ)) Rz₁w hz₁₁) $ Satisfies.formula_hereditary Rvw hv;
+  . exact Satisfies.not_of_neg (Satisfies.formula_hereditary (φ := (∼φ)) Rz₂w hz₂₁) $ Satisfies.formula_hereditary Rvw hv;
 
 end definability
 
@@ -99,7 +100,7 @@ instance [Entailment.HasAxiomKreiselPutnam 𝓢] : (canonicalFrame 𝓢).Satisfi
     by_contra hC;
     let Γx := { φ ∈ Γ | φ ∈ x.1.1};
     let Γ₁ := { φ ∈ Γ | φ ∈ ΓNyz };
-    let Γ₂ := Γ₁.preimage (∼·) $ by simp [Set.InjOn];
+    let Γ₂ := Γ₁.preimage (∼·) $ by simp [Set.InjOn, Formula.neg_inj];
     let Δy := { φ ∈ Δ | φ ∈ y.1.2};
     let Δz := { φ ∈ Δ | φ ∈ z.1.2};
     replace hC : 𝓢 ⊢ (Γx ∪ Γ₁).conj 🡒 (Δy ∪ Δz).disj := C!_replace ?_ ?_ hC;
@@ -158,7 +159,7 @@ instance [Entailment.HasAxiomKreiselPutnam 𝓢] : (canonicalFrame 𝓢).Satisfi
         rintro _ hψ ψ hψ₁ hψ₂ rfl;
         apply C!_trans CNFdisjFconj!;
         apply left_Fconj!_intro;
-        suffices ∼ψ ∈ Γ ∧ ∼ψ ∈ y.1.1 ∧ ∼ψ ∈ z.1.1 by simpa [Γ₁, Γ₂] using this;
+        suffices ∼ψ ∈ Γ ∧ ∼ψ ∈ y.1.1 ∧ ∼ψ ∈ z.1.1 by simpa [Γ₁, Γ₂, Formula.neg_inj] using this;
         tauto;
     . apply CFConj_FConj!_of_subset;
       intro φ hφ;
@@ -189,7 +190,7 @@ instance [Entailment.HasAxiomKreiselPutnam 𝓢] : (canonicalFrame 𝓢).Satisfi
       obtain ⟨Γ, Δ, hΓ, hΔ, hΓΔ⟩ := this;
       simp only [Set.subset_empty_iff, Finset.coe_eq_empty] at hΔ;
       subst hΔ;
-      simp only [Finset.disj_empty, Decidable.not_not] at hΓΔ;
+      simp only [Finset.disj_empty] at hΓΔ;
       use ({ φ ∈ Γ | φ ∈ v.1.1}).conj;
       constructor;
       . apply iff_mem₁_fconj.mpr;
@@ -216,7 +217,7 @@ instance [Entailment.HasAxiomKreiselPutnam 𝓢] : (canonicalFrame 𝓢).Satisfi
       obtain ⟨Γ, Δ, hΓ, hΔ, hΓΔ⟩ := this;
       simp only [Set.subset_empty_iff, Finset.coe_eq_empty] at hΔ;
       subst hΔ;
-      simp only [Finset.disj_empty, Decidable.not_not] at hΓΔ;
+      simp only [Finset.disj_empty] at hΓΔ;
       use ({ φ ∈ Γ | φ ∈ v.1.1}).conj;
       constructor;
       . apply iff_mem₁_fconj.mpr;
