Foundation/Propositional/Kripke/Hilbert/KC.lean
@@ -1,0 +1,159 @@
+module
+
+public import Foundation.Propositional.Kripke.AxiomWLEM
+public import Foundation.Propositional.Kripke.Hilbert.KreiselPutnam
+public import Foundation.Propositional.Kripke.Rooted
+
+@[expose] public section
+
+namespace LO.Propositional.Hilbert
+
+open Kripke
+open Formula.Kripke
+
+namespace KC
+
+instance : ({ F : Frame | F.IsPiecewiseStronglyConvergent }) ⊧* (Hilbert.KC : Hilbert ℕ) := by
+  constructor;
+  rintro φ (⟨_, rfl⟩ | ⟨_, _, _, rfl⟩) F hF <;>
+  replace hF := Set.mem_setOf_eq.mp hF;
+  . grind;
+  . exact validate_axiomWLEM_of_isPiecewiseStronglyConvergent;
+
+instance : Entailment.Consistent (Hilbert.KC : Hilbert ℕ) := consistent_of_nonempty_frameClass ({ F : Frame | F.IsPiecewiseStronglyConvergent }) $ by
+  use whitepoint;
+  apply Set.mem_setOf_eq.mpr;
+  infer_instance;
+
+instance : Canonical (Hilbert.KC : Hilbert ℕ) ({ F : Frame | F.IsPiecewiseStronglyConvergent }) := by
+  constructor;
+  apply Set.mem_setOf_eq.mpr;
+  infer_instance;
+
+instance instKripkeComplete : Complete (Hilbert.KC : Hilbert ℕ) ({ F : Frame | F.IsPiecewiseStronglyConvergent }) := inferInstance
+
+open finestFiltrationTransitiveClosureModel Relation in
+instance instKripkeCompleteFinite : Complete (Hilbert.KC : Hilbert ℕ) ({ F : Frame | Finite F ∧ F.IsPiecewiseStronglyConvergent }) := by
+  constructor;
+  intro φ hφ;
+  apply Complete.complete (𝓜 := ({ F : Frame | F.IsPiecewiseStronglyConvergent }));
+  rintro F F_conn V r;
+  replace F_conn := Set.mem_setOf_eq.mp F_conn;
+  let M : Kripke.Model := ⟨F, V⟩;
+  let RM := M↾r;
+
+  apply Model.pointGenerate.modal_equivalent_at_root (M := M) (r := r) |>.mp;
+
+  let FRM := finestFiltrationTransitiveClosureModel RM (φ.subformulas);
+  apply filtration FRM finestFiltrationTransitiveClosureModel.filterOf (by simp) |>.mpr;
+  apply hφ;
+  apply Set.mem_setOf_eq.mpr;
+  refine ⟨?_, ⟨?_⟩⟩;
+  . apply FilterEqvQuotient.finite;
+    simp;
+  . rintro X ⟨y, (rfl | Rry)⟩ ⟨z, (rfl | Rrz)⟩ RXY RXZ;
+    . simp only [exists_and_left, and_self];
+      let Z : RM.World := ⟨z, by tauto⟩;
+      use ⟦Z⟧;
+      apply Relation.TransGen.single;
+      use Z;
+      constructor;
+      . tauto;
+      . use Z;
+        constructor;
+        . tauto;
+        . apply F.refl;
+    . let Y : RM.World := ⟨y, by tauto⟩;
+      let Z : RM.World := ⟨z, by tauto⟩;
+      use ⟦Z⟧;
+      constructor;
+      . apply TransGen.single;
+        use Y, Z;
+        tauto;
+      . apply Frame.refl;
+    . let Y : RM.World := ⟨y, by tauto⟩;
+      let Z : RM.World := ⟨z, by tauto⟩;
+      use ⟦Y⟧;
+      constructor;
+      . apply Frame.refl;
+      . apply TransGen.single;
+        use Z, Y;
+        tauto;
+    . obtain ⟨u, Ryu, Rzu⟩ := F.ps_convergent Rry Rrz;
+      have : r ≺ u := F.trans Rry Ryu;
+      let Y : RM.World := ⟨y, by tauto⟩;
+      let Z : RM.World := ⟨z, by tauto⟩;
+      let U : RM.World := ⟨u, by tauto⟩;
+      use ⟦U⟧;
+      constructor;
+      . apply TransGen.single;
+        use Y, U;
+        tauto;
+      . apply TransGen.single;
+        use Z, U;
+        tauto;
+
+end KC
+
+
+instance {F : Kripke.Frame} [F.IsPiecewiseStronglyConvergent] : F.SatisfiesKreiselPutnamCondition := by
+  constructor;
+  rintro x y z ⟨Rxy, Rxz, nRyz, nRzy⟩;
+  use x;
+  refine ⟨F.refl, Rxy, Rxz, ?_⟩;
+  intro v Rxv;
+  obtain ⟨u, Ryu, Rvu⟩ := F.ps_convergent Rxy Rxv;
+  use u;
+  tauto;
+
+instance : (Hilbert.KreiselPutnam : Hilbert ℕ) ⪱ Hilbert.KC := by
+  constructor;
+  . apply weakerThan_of_subset_frameClass ({ F | F.SatisfiesKreiselPutnamCondition }) ({ F | F.IsPiecewiseStronglyConvergent });
+    apply Set.setOf_subset_setOf.mpr;
+    intro F hF;
+    infer_instance;
+  . apply Entailment.not_weakerThan_iff.mpr;
+    use Axioms.WLEM (.atom 0);
+    constructor;
+    . simp;
+    . apply Sound.not_provable_of_countermodel (𝓜 := ({ F : Frame | F.SatisfiesKreiselPutnamCondition }))
+      apply not_validOnFrameClass_of_exists_frame;
+      let F : Frame := {
+        World := Fin 3,
+        Rel := λ x y => x = 0 ∨ x = y
+        rel_partial_order := {
+          refl := by omega;
+          trans := by omega;
+          antisymm := by omega;
+        }
+      };
+      use F;
+      constructor;
+      . constructor;
+        rintro x y z ⟨Rxy, Rxz, nRyz, nRzy⟩;
+        match x, y, z with
+        | 0, 1, 2
+        | 0, 2, 1 =>
+          use 0;
+          refine ⟨by tauto, by tauto, by tauto, ?_⟩;
+          intro u hu;
+          match u with
+          | 0 => use 1; tauto;
+          | 1 => use 1; tauto;
+          | 2 => use 2; tauto;
+        | _, 0, 0
+        | _, 1, 1
+        | _, 2, 2
+        | 1, _, 2
+        | 2, _, 1
+        | 0, 0, _
+        | 0, 1, 0
+        | 0, 2, 0 => omega;
+      . apply not_imp_not.mpr $ Kripke.isPiecewiseStronglyConvergent_of_validate_axiomWLEM;
+        by_contra hC;
+        have := @F.ps_convergent _ 0 1 2;
+        omega;
+
+end LO.Propositional.Hilbert
+
+end
