Foundation/Propositional/Kripke/Hilbert/KreiselPutnam.lean
@@ -1,0 +1,109 @@
+module
+
+public import Foundation.Propositional.Kripke.AxiomKreiselPutnam
+public import Foundation.Propositional.Kripke.Hilbert.Int.Basic
+
+@[expose] public section
+
+namespace LO.Propositional.Hilbert
+
+open Kripke
+open Formula.Kripke
+
+namespace KreiselPutnam
+
+instance : ({ F : Frame | F.SatisfiesKreiselPutnamCondition }) ⊧* (Hilbert.KreiselPutnam : Hilbert ℕ) := by
+  constructor;
+  rintro φ (⟨_, rfl⟩ | ⟨_, _, _, rfl⟩) F hF <;>
+  replace hF := Set.mem_setOf_eq.mp hF;
+  . grind;
+  . exact validate_axiomKreiselPutnam_of_satisfiesKreiselPutnamCondition;
+
+instance : Entailment.Consistent (Hilbert.KreiselPutnam : Hilbert ℕ) := consistent_of_nonempty_frameClass ({ F : Frame | F.SatisfiesKreiselPutnamCondition }) $ by
+  use whitepoint;
+  apply Set.mem_setOf_eq.mpr;
+  infer_instance;
+
+instance : Canonical (Hilbert.KreiselPutnam : Hilbert ℕ) ({ F : Frame | F.SatisfiesKreiselPutnamCondition }) := by
+  constructor;
+  apply Set.mem_setOf_eq.mpr;
+  infer_instance;
+
+instance : Complete (Hilbert.KreiselPutnam : Hilbert ℕ) ({ F : Frame | F.SatisfiesKreiselPutnamCondition }) := inferInstance
+
+end KreiselPutnam
+
+instance : (Hilbert.Int : Hilbert ℕ) ⪱ Hilbert.KreiselPutnam := by
+  constructor;
+  . apply weakerThan_of_le; simp;
+  . apply Entailment.not_weakerThan_iff.mpr;
+    use Axioms.KreiselPutnam (.atom 0) (.atom 1) (.atom 2);
+    constructor;
+    . simp;
+    . apply Sound.not_provable_of_countermodel (𝓜 := FrameClass.all)
+      apply not_validOnFrameClass_of_exists_model_world;
+      let M : Kripke.Model := {
+        World := Fin 5
+        Rel x y := x = y ∨ x = 0 ∨ (x ≤ 1 ∧ y = 2) ∨ (x ≤ 1 ∧ y = 3) ∨ (x ≤ 1 ∧ y = 4)
+        rel_partial_order := {
+          refl := by tauto;
+          trans := by omega;
+          antisymm := by omega;
+        }
+        Val := ⟨λ a w =>
+          match a with
+          | 0 => w = 2
+          | 1 => w = 3
+          | 2 => w = 4
+          | _ => False,
+          by
+            intro x y Rxy a ha;
+            split at ha;
+            . subst ha; simp [Frame.Rel'] at Rxy; tauto;
+            . subst ha; simp [Frame.Rel'] at Rxy; tauto;
+            . subst ha; simp [Frame.Rel'] at Rxy; tauto;
+            . tauto;
+        ⟩
+      }
+      use M, 0;
+      constructor;
+      . tauto;
+      . apply Satisfies.imp_def.not.mpr;
+        push_neg;
+        use 1;
+        constructor;
+        . tauto;
+        . constructor;
+          . intro x R1x;
+            match x with
+            | 0 => omega;
+            | 1 =>
+              suffices ¬Satisfies M 1 (∼.atom 0) by tauto
+              apply Satisfies.neg_def.not.mpr;
+              push_neg;
+              use 2;
+              constructor;
+              . tauto;
+              . simp [Semantics.Models, Satisfies, M];
+            | 2 => tauto;
+            | 3 => tauto;
+            | 4 => tauto;
+          . apply Satisfies.or_def.not.mpr;
+            push_neg;
+            constructor;
+            . apply Satisfies.imp_def.not.mpr;
+              push_neg;
+              use 4;
+              constructor;
+              . tauto;
+              . simp [Semantics.Models, Satisfies, M, Frame.Rel'];
+            . apply Satisfies.imp_def.not.mpr;
+              push_neg;
+              use 3;
+              constructor;
+              . tauto;
+              . simp [Semantics.Models, Satisfies, M, Frame.Rel'];
+
+end LO.Propositional.Hilbert
+
+end
