Foundation/Propositional/Kripke2/Hilbert/F_Sym.lean
@@ -1,0 +1,56 @@
+module
+
+public import Foundation.Propositional.Kripke2.Hilbert.F_Ser
+public import Foundation.Propositional.Kripke2.Axiom.Sym
+
+@[expose] public section
+
+namespace LO.Propositional
+
+open Kripke2
+
+namespace Kripke2
+
+instance : trivialFrame.IsSymmetric where
+  symm := by simp
+
+end Kripke2
+
+
+namespace HilbertF.F_Sym
+
+open Kripke2
+
+instance soundKripke2 : Sound (HilbertF.F_Sym : HilbertF ℕ) ({ F | F.IsSymmetric } : Kripke2.FrameClass) := by
+  apply instFrameClassSound;
+  constructor;
+  rintro φ hφ F hF;
+  replace hF := Set.mem_setOf_eq.mp hF;
+  rcases hφ with ⟨_, _, rfl⟩;
+  simp;
+
+instance : Entailment.Consistent (HilbertF.F_Sym : HilbertF ℕ) := consistent_of_sound_frameclass soundKripke2 $ by
+  use Kripke2.trivialFrame;
+  apply Set.mem_setOf_eq.mpr;
+  infer_instance;
+
+end HilbertF.F_Sym
+
+instance : (HilbertF.F : HilbertF ℕ) ⪱ HilbertF.F_Sym := by
+  constructor;
+  . grind;
+  . apply Entailment.not_weakerThan_iff.mpr;
+    use (Axioms.Sym #0 #1);
+    constructor;
+    . simp;
+    . apply Sound.not_provable_of_countermodel (𝓜 := Kripke2.FrameClass.F);
+      apply Kripke2.not_validOnFrameClass_of_exists_frame;
+      use ⟨Fin 2, (λ x y => x < y ∨ x = 0), 0, by simp⟩;
+      constructor;
+      . tauto;
+      . by_contra hC;
+        have := isSymmetric_of_valid_axiomSym hC |>.symm 0 1;
+        simp at this;
+
+end LO.Propositional
+end
