Foundation/Propositional/Kripke2/Hilbert/F_Tra1.lean
@@ -1,0 +1,69 @@
+module
+
+public import Foundation.Propositional.Kripke2.Hilbert.F_Ser
+public import Foundation.Propositional.Kripke2.Axiom.Tra
+
+@[expose] public section
+
+namespace LO.Propositional
+
+open Kripke2
+
+
+namespace Kripke2
+
+protected abbrev FrameClass.F_Tra1 : Kripke2.FrameClass := { F | F.IsTransitive }
+
+instance : trivialFrame.IsTransitive where
+  trans := by simp
+
+end Kripke2
+
+
+namespace HilbertF.F_Tra1
+
+open Kripke2
+
+instance soundKripke2 : Sound (HilbertF.F_Tra1 : HilbertF ℕ) ({ F | F.IsTransitive } : Kripke2.FrameClass) := by
+  apply instFrameClassSound;
+  constructor;
+  rintro φ hφ F hF;
+  replace hF := Set.mem_setOf_eq.mp hF;
+  rcases hφ with ⟨_, _, _, rfl⟩;
+  simp;
+
+instance : Entailment.Consistent (HilbertF.F_Tra1 : HilbertF ℕ) := consistent_of_sound_frameclass soundKripke2 $ by
+  use Kripke2.trivialFrame;
+  apply Set.mem_setOf_eq.mpr;
+  infer_instance;
+
+/-
+instance Kripke2.complete : Complete Propositional.F_Tra1 FrameClass.F_Tra1 := by
+  constructor;
+  intro φ hφ;
+  apply Kripke2.provable_of_validOncanonicalModel;
+  apply hφ;
+  apply Set.mem_setOf_eq.mpr;
+  infer_instance;
+-/
+
+end HilbertF.F_Tra1
+
+instance : (HilbertF.F : HilbertF ℕ) ⪱ HilbertF.F_Tra1 := by
+  constructor;
+  . grind;
+  . apply Entailment.not_weakerThan_iff.mpr;
+    use (Axioms.Tra1 #0 #1 #2);
+    constructor;
+    . simp;
+    . apply Sound.not_provable_of_countermodel (𝓜 := Kripke2.FrameClass.F);
+      apply Kripke2.not_validOnFrameClass_of_exists_frame;
+      use ⟨Fin 2, (λ x y => x = 0 ∨ x ≠ y), 0, by simp⟩;
+      constructor;
+      . tauto;
+      . by_contra hC;
+        simpa using IsTransitive_of_valid_axiomTra₁ hC |>.trans 1;
+
+
+end LO.Propositional
+end
